driver/Complements.v
@@ -17,6 +17,7 @@ Require Import Coqlib Errors.
 Require Import AST Linking Events Smallstep Behaviors.
 Require Import Csyntax Csem Cstrategy Asm.
 Require Import Compiler.
+Require Import Clight.
 
 (** * Preservation of whole-program behaviors *)
 
@@ -38,6 +39,14 @@ Proof.
   apply transf_c_program_correct; auto.
 Qed.
 
+Theorem transf_clight_program_preservation:
+  forall p tp beh,
+  transf_clight_program p = OK tp ->
+  program_behaves (Asm.semantics tp) beh ->
+  exists beh', program_behaves (Clight.semantics2 p) beh' /\ behavior_improves beh' beh.
+Proof.
+Admitted.
+
 (** As a corollary, if the source C code cannot go wrong, i.e. is free of
   undefined behaviors, the behavior of the generated assembly code is
   one of the possible behaviors of the source C code. *)
@@ -51,6 +60,14 @@ Proof.
   intros. eapply backward_simulation_same_safe_behavior; eauto.
   apply transf_c_program_correct; auto.
 Qed.
+
+Theorem transf_clight_program_is_refinement:
+  forall p tp,
+  transf_clight_program p = OK tp ->
+  (forall beh, program_behaves (Clight.semantics2 p) beh -> not_wrong beh) ->
+  (forall beh, program_behaves (Asm.semantics tp) beh -> program_behaves (Clight.semantics2 p) beh).
+Proof.
+Admitted. 
 
 (** If we consider the C evaluation strategy implemented by the compiler,
   we get stronger preservation results. *)
@@ -134,6 +151,8 @@ Definition specification := program_behavior -> Prop.
 
 Definition c_program_satisfies_spec (p: Csyntax.program) (spec: specification): Prop :=
   forall beh,  program_behaves (Csem.semantics p) beh -> spec beh.
+Definition clight_program_satisfies_spec (p: Clight.program) (spec: specification): Prop :=
+  forall beh,  program_behaves (Clight.semantics2 p) beh -> spec beh.
 Definition asm_program_satisfies_spec (p: Asm.program) (spec: specification): Prop :=
   forall beh,  program_behaves (Asm.semantics p) beh -> spec beh.
   
@@ -302,3 +321,73 @@ Proof.
 Qed.
 
 End SEPARATE_COMPILATION.
+
+Section CLIGHT_SEPARATE_COMPILATION.
+
+(** The source: a list of C compilation units *)
+Variable c_units: nlist Clight.program.
+
+(** The compiled code: a list of Asm compilation units, obtained by separate compilation *)
+Variable asm_units: nlist Asm.program.
+Hypothesis separate_compilation_succeeds: 
+  nlist_forall2 (fun cu tcu => transf_clight_program cu = OK tcu) c_units asm_units.
+
+(** We assume that the source C compilation units can be linked together
+    to obtain a monolithic C program [c_program]. *)
+Variable c_program: Clight.program.
+Hypothesis source_linking: link_list c_units = Some c_program.
+
+(** Then, linking the Asm units obtained by separate compilation succeeds. *)
+Lemma clight_compiled_linking_succeeds:
+  { asm_program | link_list asm_units = Some asm_program }.
+Proof.
+Admitted.
+
+(** Let asm_program be the result of linking the Asm units. *)
+Let asm_program: Asm.program := proj1_sig clight_compiled_linking_succeeds.
+Let compiled_linking: link_list asm_units = Some asm_program := proj2_sig clight_compiled_linking_succeeds.
+
+(** Then, [asm_program] preserves the semantics and the specifications of
+  [c_program], in the following sense.
+  First, every behavior of [asm_program] improves upon one of the possible
+  behaviors of [c_program]. *)
+
+Theorem separate_transf_clight_program_preservation:
+  forall beh,
+  program_behaves (Asm.semantics asm_program) beh ->
+  exists beh', program_behaves (Clight.semantics2 c_program) beh' /\ behavior_improves beh' beh.
+Proof.
+Admitted.
+
+(** As a corollary, if [c_program] is free of undefined behaviors, 
+  the behavior of [asm_program] is one of the possible behaviors of [c_program]. *)
+
+Theorem separate_transf_clight_program_is_refinement:
+  (forall beh, program_behaves (Clight.semantics2 c_program) beh -> not_wrong beh) ->
+  (forall beh, program_behaves (Asm.semantics asm_program) beh -> program_behaves (Clight.semantics2 c_program) beh).
+Proof.
+  intros. exploit separate_transf_clight_program_preservation; eauto. intros (beh' & P & Q).
+  assert (not_wrong beh') by auto.
+  inv Q.
+- auto.
+- destruct H2 as (t & U & V). subst beh'. elim H1. 
+Qed.
+
+(** We now show that if all executions of [c_program] satisfy a specification,
+  then all executions of [asm_program] also satisfy the specification, provided
+  the specification is of the safety-enforcing kind. *)
+
+Theorem separate_transf_clight_program_preserves_spec:
+  forall spec,
+  safety_enforcing_specification spec ->
+  clight_program_satisfies_spec c_program spec ->
+  asm_program_satisfies_spec asm_program spec.
+Proof.
+  intros spec SES CSAT; red; intros beh AEXEC.
+  exploit separate_transf_clight_program_preservation; eauto. intros (beh' & CEXEC & IMPR).
+  apply CSAT in CEXEC. destruct IMPR as [EQ | [t [A B]]].
+- congruence.
+- subst beh'. apply SES in CEXEC. contradiction. 
+Qed.
+
+End CLIGHT_SEPARATE_COMPILATION.
