stanfrontend/Scompiler.v
@@ -1,0 +1,13 @@
+Require Import Stan.
+Require Import Clight.
+Require Import Errors.
+Require Import Smallstep.
+
+Parameter transf_stan_program: Stan.program -> res Clight.program.
+
+Theorem transf_stan_program_correct:
+  forall p tp,
+  transf_stan_program p = OK tp ->
+  backward_simulation (Stan.semantics p) (Clight.semantics2 tp).
+Proof.
+Admitted.
